src3.0/Vellvm/vellvm_tactics.v
@@ -1,4 +1,7 @@
 Require Import Coqlib.
+Require Import Metatheory.
+
+Ltac tinv H := try solve [inv H].
 
 Ltac uniq_result :=
 repeat match goal with
@@ -20,5 +23,154 @@ repeat match goal with
 | H : ?f _ _ _ _ = ?f _ _ _ _ |- _ => inv H
 | H : ?f _ _ _ _ _ = ?f _ _ _ _ _ |- _ => inv H
 | H : False |- _ => inv H
+end.
+
+Ltac destruct_if :=
+match goal with
+| H: context [(if ?lk then _ else _)] |- _ =>
+   remember lk as R; destruct R; try inv H
+| H: context [if ?lk then _ else _] |- _ =>
+   remember lk as R; destruct R; try inv H
+end.
+
+Ltac destruct_let :=
+  match goal with
+  | _: context [match ?e with 
+                | (_,_) => _
+                end] |- _ => destruct e
+  | |- context [match ?e with 
+                | (_,_) => _
+                end] => destruct e
+  end.
+
+Ltac destruct_exists :=
+repeat match goal with
+| H : exists _, _ |- _ =>
+    let A := fresh "A" in
+    let J := fresh "J" in
+    destruct H as [A J]
+end.
+
+Ltac destruct_ands :=
+repeat match goal with
+| H : _ /\ _ |- _ => destruct H
+end.
+
+Ltac zeauto := eauto with zarith.
+
+Ltac inv_mbind :=
+  repeat match goal with
+         | H : match ?e with
+               | Some _ => _
+               | None => None
+               end = Some _ |- _ => remember e as R; destruct R as [|]; inv H
+         | H : Some _ = match ?e with
+               | Some _ => _
+               | None => None
+               end |- _ => remember e as R; destruct R as [|]; inv H
+         | H :  Some _ = match ?p with
+                        | (_, _) => _
+                        end |- _ => destruct p
+         | H : if ?e then _ else False |- _ =>
+             remember e as R; destruct R; tinv H
+         | H : if ?e then False else _ |- _ =>
+             remember e as R; destruct R; tinv H
+         end.
+
+Ltac inv_mbind' := inv_mbind.
+Ltac inv_mbind'' := inv_mbind.
+
+Ltac solve_in_prefix :=
+repeat match goal with
+| G: In ?i (?prefix ++ _) |- In ?i (?prefix ++ _) =>
+  apply in_or_app;
+  apply in_app_or in G;
+  destruct G as [G | G]; auto;
+  right
+end.
+
+Ltac solve_in_head :=
+match goal with
+| H0 : In _ ([_] ++ _),
+  J2 : _ \/ _ \/ _ |- _ =>
+    simpl in H0;
+    destruct H0 as [H0 | H0]; subst; try solve [
+      destruct J2 as [J2 | [J2 | J2]]; subst;
+        repeat match goal with
+        | H : _ /\ _ |- _ => destruct H
+        end; congruence]
+| H0 : In _ (_:: _),
+  J2 : _ \/ _ \/ _ |- _ =>
+    simpl in H0;
+    destruct H0 as [H0 | H0]; subst; try solve [
+      destruct J2 as [J2 | [J2 | J2]]; subst;
+        repeat match goal with
+        | H : _ /\ _ |- _ => destruct H
+        end; congruence]
+| H0 : _ = _ \/ In _ _,
+  J2 : _ \/ _ \/ _ |- _ =>
+    simpl in H0;
+    destruct H0 as [H0 | H0]; subst; try solve [
+      destruct J2 as [J2 | [J2 | J2]]; subst;
+        repeat match goal with
+        | H : _ /\ _ |- _ => destruct H
+        end; congruence]
+end.
+
+Ltac zauto := auto with zarith.
+
+Ltac SSSSSCase name := Case_aux subsubsubsubsubcase name.
+Ltac SSSSSSCase name := Case_aux subsubsubsubsubsubcase name.
+
+Ltac tac0 := match goal with
+  | |- exists _, _ => idtac
+  | |- _ => solve [eauto]
+  end.
+
+
+Ltac symmetry_ctx :=
+  repeat match goal with
+  | H : Some _ = _ |- _ => symmetry in H
+  end.
+
+Ltac app_inv :=
+  repeat match goal with
+  | [ H: Some _ = Some _ |- _ ] => inv H
+  end.
+
+Ltac trans_eq :=
+  repeat match goal with
+  | H1 : ?a = ?b, H2 : ?c = ?b |- _ => rewrite <- H1 in H2; inv H2
+  | H1 : ?a = ?b, H2 : ?b = ?c |- _ => rewrite <- H1 in H2; inv H2
+  end.
+
+Ltac inv_mfalse :=
+  repeat match goal with
+         | H : match ?e with
+               | Some _ => _
+               | None => False
+               end |- _ => remember e as R; destruct R as [|]; tinv H
+         end.
+
+Tactic Notation "binvt" ident(H) "as" ident(J1) ident(J2) :=
+apply orb_true_iff in H; destruct H as [J1 | J2].
+
+Tactic Notation "binvf" ident(H) "as" ident(J1) ident(J2) :=
+apply orb_false_iff in H; destruct H as [J1 J2].
+
+Ltac destruct_match :=
+match goal with
+| H: match ?lk with
+     | Some _ => Some _
+     | None => _
+     end = Some _ |- _ => 
+   let r := fresh "r" in
+   remember lk as R; destruct R as [r|]; inv H; symmetry_ctx
+end.
+
+Ltac fill_ctxhole :=
+match goal with
+| H : ?e = _ |- context [ ?e ] => rewrite H
+| H : _ = ?e |- context [ ?e ] => rewrite H
 end.
 
